ocaml/fstar-lib/generated/FStar_Interactive_Ide_Types.ml
@@ -3,28 +3,6 @@ let (initial_range : FStar_Compiler_Range.range) =
   let uu___ = FStar_Compiler_Range.mk_pos Prims.int_one Prims.int_zero in
   let uu___1 = FStar_Compiler_Range.mk_pos Prims.int_one Prims.int_zero in
   FStar_Compiler_Range.mk_range "<input>" uu___ uu___1
-let (js_pushkind :
-  FStar_Compiler_Util.json -> FStar_Interactive_PushHelper.push_kind) =
-  fun s ->
-    let uu___ = FStar_Interactive_JsonHelper.js_str s in
-    match uu___ with
-    | "syntax" -> FStar_Interactive_PushHelper.SyntaxCheck
-    | "lax" -> FStar_Interactive_PushHelper.LaxCheck
-    | "full" -> FStar_Interactive_PushHelper.FullCheck
-    | uu___1 -> FStar_Interactive_JsonHelper.js_fail "push_kind" s
-let (js_reductionrule :
-  FStar_Compiler_Util.json -> FStar_TypeChecker_Env.step) =
-  fun s ->
-    let uu___ = FStar_Interactive_JsonHelper.js_str s in
-    match uu___ with
-    | "beta" -> FStar_TypeChecker_Env.Beta
-    | "delta" ->
-        FStar_TypeChecker_Env.UnfoldUntil FStar_Syntax_Syntax.delta_constant
-    | "iota" -> FStar_TypeChecker_Env.Iota
-    | "zeta" -> FStar_TypeChecker_Env.Zeta
-    | "reify" -> FStar_TypeChecker_Env.Reify
-    | "pure-subterms" -> FStar_TypeChecker_Env.PureSubtermsWithinComputations
-    | uu___1 -> FStar_Interactive_JsonHelper.js_fail "reduction rule" s
 type completion_context =
   | CKCode 
   | CKOption of Prims.bool 
@@ -42,28 +20,6 @@ let (uu___is_CKModuleOrNamespace : completion_context -> Prims.bool) =
 let (__proj__CKModuleOrNamespace__item___0 :
   completion_context -> (Prims.bool * Prims.bool)) =
   fun projectee -> match projectee with | CKModuleOrNamespace _0 -> _0
-let (js_optional_completion_context :
-  FStar_Compiler_Util.json FStar_Pervasives_Native.option ->
-    completion_context)
-  =
-  fun k ->
-    match k with
-    | FStar_Pervasives_Native.None -> CKCode
-    | FStar_Pervasives_Native.Some k1 ->
-        let uu___ = FStar_Interactive_JsonHelper.js_str k1 in
-        (match uu___ with
-         | "symbol" -> CKCode
-         | "code" -> CKCode
-         | "set-options" -> CKOption false
-         | "reset-options" -> CKOption true
-         | "open" -> CKModuleOrNamespace (true, true)
-         | "let-open" -> CKModuleOrNamespace (true, true)
-         | "include" -> CKModuleOrNamespace (true, false)
-         | "module-alias" -> CKModuleOrNamespace (true, false)
-         | uu___1 ->
-             FStar_Interactive_JsonHelper.js_fail
-               "completion context (code, set-options, reset-options, open, let-open, include, module-alias)"
-               k1)
 type lookup_context =
   | LKSymbolOnly 
   | LKModule 
@@ -78,63 +34,52 @@ let (uu___is_LKOption : lookup_context -> Prims.bool) =
   fun projectee -> match projectee with | LKOption -> true | uu___ -> false
 let (uu___is_LKCode : lookup_context -> Prims.bool) =
   fun projectee -> match projectee with | LKCode -> true | uu___ -> false
-let (js_optional_lookup_context :
-  FStar_Compiler_Util.json FStar_Pervasives_Native.option -> lookup_context)
-  =
-  fun k ->
-    match k with
-    | FStar_Pervasives_Native.None -> LKSymbolOnly
-    | FStar_Pervasives_Native.Some k1 ->
-        let uu___ = FStar_Interactive_JsonHelper.js_str k1 in
-        (match uu___ with
-         | "symbol-only" -> LKSymbolOnly
-         | "code" -> LKCode
-         | "set-options" -> LKOption
-         | "reset-options" -> LKOption
-         | "open" -> LKModule
-         | "let-open" -> LKModule
-         | "include" -> LKModule
-         | "module-alias" -> LKModule
-         | uu___1 ->
-             FStar_Interactive_JsonHelper.js_fail
-               "lookup context (symbol-only, code, set-options, reset-options, open, let-open, include, module-alias)"
-               k1)
 type position = (Prims.string * Prims.int * Prims.int)
+type push_kind =
+  | SyntaxCheck 
+  | LaxCheck 
+  | FullCheck 
+let (uu___is_SyntaxCheck : push_kind -> Prims.bool) =
+  fun projectee ->
+    match projectee with | SyntaxCheck -> true | uu___ -> false
+let (uu___is_LaxCheck : push_kind -> Prims.bool) =
+  fun projectee -> match projectee with | LaxCheck -> true | uu___ -> false
+let (uu___is_FullCheck : push_kind -> Prims.bool) =
+  fun projectee -> match projectee with | FullCheck -> true | uu___ -> false
 type push_query =
   {
-  push_kind: FStar_Interactive_PushHelper.push_kind ;
+  push_kind: push_kind ;
   push_line: Prims.int ;
   push_column: Prims.int ;
   push_peek_only: Prims.bool ;
   push_code_or_decl:
     (Prims.string, FStar_Parser_AST.decl) FStar_Pervasives.either }
-let (__proj__Mkpush_query__item__push_kind :
-  push_query -> FStar_Interactive_PushHelper.push_kind) =
+let (__proj__Mkpush_query__item__push_kind : push_query -> push_kind) =
   fun projectee ->
     match projectee with
-    | { push_kind; push_line; push_column; push_peek_only;
-        push_code_or_decl;_} -> push_kind
+    | { push_kind = push_kind1; push_line; push_column; push_peek_only;
+        push_code_or_decl;_} -> push_kind1
 let (__proj__Mkpush_query__item__push_line : push_query -> Prims.int) =
   fun projectee ->
     match projectee with
-    | { push_kind; push_line; push_column; push_peek_only;
+    | { push_kind = push_kind1; push_line; push_column; push_peek_only;
         push_code_or_decl;_} -> push_line
 let (__proj__Mkpush_query__item__push_column : push_query -> Prims.int) =
   fun projectee ->
     match projectee with
-    | { push_kind; push_line; push_column; push_peek_only;
+    | { push_kind = push_kind1; push_line; push_column; push_peek_only;
         push_code_or_decl;_} -> push_column
 let (__proj__Mkpush_query__item__push_peek_only : push_query -> Prims.bool) =
   fun projectee ->
     match projectee with
-    | { push_kind; push_line; push_column; push_peek_only;
+    | { push_kind = push_kind1; push_line; push_column; push_peek_only;
         push_code_or_decl;_} -> push_peek_only
 let (__proj__Mkpush_query__item__push_code_or_decl :
   push_query -> (Prims.string, FStar_Parser_AST.decl) FStar_Pervasives.either)
   =
   fun projectee ->
     match projectee with
-    | { push_kind; push_line; push_column; push_peek_only;
+    | { push_kind = push_kind1; push_line; push_column; push_peek_only;
         push_code_or_decl;_} -> push_code_or_decl
 type lookup_symbol_range = FStar_Compiler_Util.json
 type query_status =
@@ -148,11 +93,64 @@ let (uu___is_QueryNOK : query_status -> Prims.bool) =
 let (uu___is_QueryViolatesProtocol : query_status -> Prims.bool) =
   fun projectee ->
     match projectee with | QueryViolatesProtocol -> true | uu___ -> false
-type callback_t =
-  FStar_Interactive_ReplState.repl_state ->
-    ((query_status * FStar_Compiler_Util.json Prims.list) *
-      (FStar_Interactive_ReplState.repl_state, Prims.int)
+type repl_depth_t = (FStar_TypeChecker_Env.tcenv_depth_t * Prims.int)
+type optmod_t = FStar_Syntax_Syntax.modul FStar_Pervasives_Native.option
+type timed_fname =
+  {
+  tf_fname: Prims.string ;
+  tf_modtime: FStar_Compiler_Util.time }
+let (__proj__Mktimed_fname__item__tf_fname : timed_fname -> Prims.string) =
+  fun projectee ->
+    match projectee with | { tf_fname; tf_modtime;_} -> tf_fname
+let (__proj__Mktimed_fname__item__tf_modtime :
+  timed_fname -> FStar_Compiler_Util.time) =
+  fun projectee ->
+    match projectee with | { tf_fname; tf_modtime;_} -> tf_modtime
+type repl_task =
+  | LDInterleaved of (timed_fname * timed_fname) 
+  | LDSingle of timed_fname 
+  | LDInterfaceOfCurrentFile of timed_fname 
+  | PushFragment of (FStar_Parser_ParseIt.input_frag, FStar_Parser_AST.decl)
+  FStar_Pervasives.either 
+  | Noop 
+let (uu___is_LDInterleaved : repl_task -> Prims.bool) =
+  fun projectee ->
+    match projectee with | LDInterleaved _0 -> true | uu___ -> false
+let (__proj__LDInterleaved__item___0 :
+  repl_task -> (timed_fname * timed_fname)) =
+  fun projectee -> match projectee with | LDInterleaved _0 -> _0
+let (uu___is_LDSingle : repl_task -> Prims.bool) =
+  fun projectee ->
+    match projectee with | LDSingle _0 -> true | uu___ -> false
+let (__proj__LDSingle__item___0 : repl_task -> timed_fname) =
+  fun projectee -> match projectee with | LDSingle _0 -> _0
+let (uu___is_LDInterfaceOfCurrentFile : repl_task -> Prims.bool) =
+  fun projectee ->
+    match projectee with
+    | LDInterfaceOfCurrentFile _0 -> true
+    | uu___ -> false
+let (__proj__LDInterfaceOfCurrentFile__item___0 : repl_task -> timed_fname) =
+  fun projectee -> match projectee with | LDInterfaceOfCurrentFile _0 -> _0
+let (uu___is_PushFragment : repl_task -> Prims.bool) =
+  fun projectee ->
+    match projectee with | PushFragment _0 -> true | uu___ -> false
+let (__proj__PushFragment__item___0 :
+  repl_task ->
+    (FStar_Parser_ParseIt.input_frag, FStar_Parser_AST.decl)
       FStar_Pervasives.either)
+  = fun projectee -> match projectee with | PushFragment _0 -> _0
+let (uu___is_Noop : repl_task -> Prims.bool) =
+  fun projectee -> match projectee with | Noop -> true | uu___ -> false
+type full_buffer_request_kind =
+  | Full 
+  | Cache 
+  | ReloadDeps 
+let (uu___is_Full : full_buffer_request_kind -> Prims.bool) =
+  fun projectee -> match projectee with | Full -> true | uu___ -> false
+let (uu___is_Cache : full_buffer_request_kind -> Prims.bool) =
+  fun projectee -> match projectee with | Cache -> true | uu___ -> false
+let (uu___is_ReloadDeps : full_buffer_request_kind -> Prims.bool) =
+  fun projectee -> match projectee with | ReloadDeps -> true | uu___ -> false
 type query' =
   | Exit 
   | DescribeProtocol 
@@ -170,12 +168,28 @@ type query' =
   | Search of Prims.string 
   | GenericError of Prims.string 
   | ProtocolViolation of Prims.string 
-  | FullBuffer of (Prims.string * Prims.bool) 
-  | Callback of callback_t 
+  | FullBuffer of (Prims.string * full_buffer_request_kind) 
+  | Callback of
+  (repl_state ->
+     ((query_status * FStar_Compiler_Util.json Prims.list) * (repl_state,
+       Prims.int) FStar_Pervasives.either))
+  
   | Format of Prims.string 
+  | Cancel of position FStar_Pervasives_Native.option 
 and query = {
   qq: query' ;
   qid: Prims.string }
+and repl_state =
+  {
+  repl_line: Prims.int ;
+  repl_column: Prims.int ;
+  repl_fname: Prims.string ;
+  repl_deps_stack: (repl_depth_t * (repl_task * repl_state)) Prims.list ;
+  repl_curmod: optmod_t ;
+  repl_env: FStar_TypeChecker_Env.env ;
+  repl_stdin: FStar_Compiler_Util.stream_reader ;
+  repl_names: FStar_Interactive_CompletionTable.table ;
+  repl_buffered_input_queries: query Prims.list }
 let (uu___is_Exit : query' -> Prims.bool) =
   fun projectee -> match projectee with | Exit -> true | uu___ -> false
 let (uu___is_DescribeProtocol : query' -> Prims.bool) =
@@ -237,28 +251,182 @@ let (__proj__ProtocolViolation__item___0 : query' -> Prims.string) =
 let (uu___is_FullBuffer : query' -> Prims.bool) =
   fun projectee ->
     match projectee with | FullBuffer _0 -> true | uu___ -> false
-let (__proj__FullBuffer__item___0 : query' -> (Prims.string * Prims.bool)) =
+let (__proj__FullBuffer__item___0 :
+  query' -> (Prims.string * full_buffer_request_kind)) =
   fun projectee -> match projectee with | FullBuffer _0 -> _0
 let (uu___is_Callback : query' -> Prims.bool) =
   fun projectee ->
     match projectee with | Callback _0 -> true | uu___ -> false
-let (__proj__Callback__item___0 : query' -> callback_t) =
-  fun projectee -> match projectee with | Callback _0 -> _0
+let (__proj__Callback__item___0 :
+  query' ->
+    repl_state ->
+      ((query_status * FStar_Compiler_Util.json Prims.list) * (repl_state,
+        Prims.int) FStar_Pervasives.either))
+  = fun projectee -> match projectee with | Callback _0 -> _0
 let (uu___is_Format : query' -> Prims.bool) =
   fun projectee -> match projectee with | Format _0 -> true | uu___ -> false
 let (__proj__Format__item___0 : query' -> Prims.string) =
   fun projectee -> match projectee with | Format _0 -> _0
+let (uu___is_Cancel : query' -> Prims.bool) =
+  fun projectee -> match projectee with | Cancel _0 -> true | uu___ -> false
+let (__proj__Cancel__item___0 :
+  query' -> position FStar_Pervasives_Native.option) =
+  fun projectee -> match projectee with | Cancel _0 -> _0
 let (__proj__Mkquery__item__qq : query -> query') =
   fun projectee -> match projectee with | { qq; qid;_} -> qq
 let (__proj__Mkquery__item__qid : query -> Prims.string) =
   fun projectee -> match projectee with | { qq; qid;_} -> qid
+let (__proj__Mkrepl_state__item__repl_line : repl_state -> Prims.int) =
+  fun projectee ->
+    match projectee with
+    | { repl_line; repl_column; repl_fname; repl_deps_stack; repl_curmod;
+        repl_env; repl_stdin; repl_names; repl_buffered_input_queries;_} ->
+        repl_line
+let (__proj__Mkrepl_state__item__repl_column : repl_state -> Prims.int) =
+  fun projectee ->
+    match projectee with
+    | { repl_line; repl_column; repl_fname; repl_deps_stack; repl_curmod;
+        repl_env; repl_stdin; repl_names; repl_buffered_input_queries;_} ->
+        repl_column
+let (__proj__Mkrepl_state__item__repl_fname : repl_state -> Prims.string) =
+  fun projectee ->
+    match projectee with
+    | { repl_line; repl_column; repl_fname; repl_deps_stack; repl_curmod;
+        repl_env; repl_stdin; repl_names; repl_buffered_input_queries;_} ->
+        repl_fname
+let (__proj__Mkrepl_state__item__repl_deps_stack :
+  repl_state -> (repl_depth_t * (repl_task * repl_state)) Prims.list) =
+  fun projectee ->
+    match projectee with
+    | { repl_line; repl_column; repl_fname; repl_deps_stack; repl_curmod;
+        repl_env; repl_stdin; repl_names; repl_buffered_input_queries;_} ->
+        repl_deps_stack
+let (__proj__Mkrepl_state__item__repl_curmod : repl_state -> optmod_t) =
+  fun projectee ->
+    match projectee with
+    | { repl_line; repl_column; repl_fname; repl_deps_stack; repl_curmod;
+        repl_env; repl_stdin; repl_names; repl_buffered_input_queries;_} ->
+        repl_curmod
+let (__proj__Mkrepl_state__item__repl_env :
+  repl_state -> FStar_TypeChecker_Env.env) =
+  fun projectee ->
+    match projectee with
+    | { repl_line; repl_column; repl_fname; repl_deps_stack; repl_curmod;
+        repl_env; repl_stdin; repl_names; repl_buffered_input_queries;_} ->
+        repl_env
+let (__proj__Mkrepl_state__item__repl_stdin :
+  repl_state -> FStar_Compiler_Util.stream_reader) =
+  fun projectee ->
+    match projectee with
+    | { repl_line; repl_column; repl_fname; repl_deps_stack; repl_curmod;
+        repl_env; repl_stdin; repl_names; repl_buffered_input_queries;_} ->
+        repl_stdin
+let (__proj__Mkrepl_state__item__repl_names :
+  repl_state -> FStar_Interactive_CompletionTable.table) =
+  fun projectee ->
+    match projectee with
+    | { repl_line; repl_column; repl_fname; repl_deps_stack; repl_curmod;
+        repl_env; repl_stdin; repl_names; repl_buffered_input_queries;_} ->
+        repl_names
+let (__proj__Mkrepl_state__item__repl_buffered_input_queries :
+  repl_state -> query Prims.list) =
+  fun projectee ->
+    match projectee with
+    | { repl_line; repl_column; repl_fname; repl_deps_stack; repl_curmod;
+        repl_env; repl_stdin; repl_names; repl_buffered_input_queries;_} ->
+        repl_buffered_input_queries
+type callback_t =
+  repl_state ->
+    ((query_status * FStar_Compiler_Util.json Prims.list) * (repl_state,
+      Prims.int) FStar_Pervasives.either)
+type repl_stack_entry_t = (repl_depth_t * (repl_task * repl_state))
+type repl_stack_t = (repl_depth_t * (repl_task * repl_state)) Prims.list
+type grepl_state =
+  {
+  grepl_repls: repl_state FStar_Compiler_Util.psmap ;
+  grepl_stdin: FStar_Compiler_Util.stream_reader }
+let (__proj__Mkgrepl_state__item__grepl_repls :
+  grepl_state -> repl_state FStar_Compiler_Util.psmap) =
+  fun projectee ->
+    match projectee with | { grepl_repls; grepl_stdin;_} -> grepl_repls
+let (__proj__Mkgrepl_state__item__grepl_stdin :
+  grepl_state -> FStar_Compiler_Util.stream_reader) =
+  fun projectee ->
+    match projectee with | { grepl_repls; grepl_stdin;_} -> grepl_stdin
+let (t0 : FStar_Compiler_Util.time) = FStar_Compiler_Util.now ()
+let (dummy_tf_of_fname : Prims.string -> timed_fname) =
+  fun fname -> { tf_fname = fname; tf_modtime = t0 }
+let (string_of_timed_fname : timed_fname -> Prims.string) =
+  fun uu___ ->
+    match uu___ with
+    | { tf_fname = fname; tf_modtime = modtime;_} ->
+        if modtime = t0
+        then FStar_Compiler_Util.format1 "{ %s }" fname
+        else
+          (let uu___2 = FStar_Compiler_Util.string_of_time modtime in
+           FStar_Compiler_Util.format2 "{ %s; %s }" fname uu___2)
+let (string_of_repl_task : repl_task -> Prims.string) =
+  fun uu___ ->
+    match uu___ with
+    | LDInterleaved (intf, impl) ->
+        let uu___1 = string_of_timed_fname intf in
+        let uu___2 = string_of_timed_fname impl in
+        FStar_Compiler_Util.format2 "LDInterleaved (%s, %s)" uu___1 uu___2
+    | LDSingle intf_or_impl ->
+        let uu___1 = string_of_timed_fname intf_or_impl in
+        FStar_Compiler_Util.format1 "LDSingle %s" uu___1
+    | LDInterfaceOfCurrentFile intf ->
+        let uu___1 = string_of_timed_fname intf in
+        FStar_Compiler_Util.format1 "LDInterfaceOfCurrentFile %s" uu___1
+    | PushFragment (FStar_Pervasives.Inl frag) ->
+        FStar_Compiler_Util.format1 "PushFragment { code = %s }"
+          frag.FStar_Parser_ParseIt.frag_text
+    | PushFragment (FStar_Pervasives.Inr d) ->
+        let uu___1 = FStar_Parser_AST.decl_to_string d in
+        FStar_Compiler_Util.format1 "PushFragment { decl = %s }" uu___1
+    | Noop -> "Noop {}"
+let (string_of_repl_stack_entry : repl_stack_entry_t -> Prims.string) =
+  fun uu___ ->
+    match uu___ with
+    | ((depth, i), (task, state)) ->
+        let uu___1 =
+          let uu___2 = FStar_Compiler_Util.string_of_int i in
+          let uu___3 = let uu___4 = string_of_repl_task task in [uu___4] in
+          uu___2 :: uu___3 in
+        FStar_Compiler_Util.format "{depth=%s; task=%s}" uu___1
+let (string_of_repl_stack : repl_stack_entry_t Prims.list -> Prims.string) =
+  fun s ->
+    let uu___ = FStar_Compiler_List.map string_of_repl_stack_entry s in
+    FStar_String.concat ";\n\t\t" uu___
+let (repl_state_to_string : repl_state -> Prims.string) =
+  fun r ->
+    let uu___ =
+      let uu___1 = FStar_Compiler_Util.string_of_int r.repl_line in
+      let uu___2 =
+        let uu___3 = FStar_Compiler_Util.string_of_int r.repl_column in
+        let uu___4 =
+          let uu___5 =
+            let uu___6 =
+              match r.repl_curmod with
+              | FStar_Pervasives_Native.None -> "None"
+              | FStar_Pervasives_Native.Some m ->
+                  FStar_Ident.string_of_lid m.FStar_Syntax_Syntax.name in
+            let uu___7 =
+              let uu___8 = string_of_repl_stack r.repl_deps_stack in [uu___8] in
+            uu___6 :: uu___7 in
+          (r.repl_fname) :: uu___5 in
+        uu___3 :: uu___4 in
+      uu___1 :: uu___2 in
+    FStar_Compiler_Util.format
+      "{\n\trepl_line=%s;\n\trepl_column=%s;\n\trepl_fname=%s;\n\trepl_cur_mod=%s;\n\t\\      \r\n      repl_deps_stack={%s}\n}"
+      uu___
 let (push_query_to_string : push_query -> Prims.string) =
   fun pq ->
     let pk =
       match pq.push_kind with
-      | FStar_Interactive_PushHelper.SyntaxCheck -> "SyntaxCheck"
-      | FStar_Interactive_PushHelper.LaxCheck -> "LaxCheck"
-      | FStar_Interactive_PushHelper.FullCheck -> "FullCheck" in
+      | SyntaxCheck -> "SyntaxCheck"
+      | LaxCheck -> "LaxCheck"
+      | FullCheck -> "FullCheck" in
     let code_or_decl =
       match pq.push_code_or_decl with
       | FStar_Pervasives.Inl code -> code
@@ -299,6 +467,7 @@ let (query_to_string : query -> Prims.string) =
     | FullBuffer uu___ -> "FullBuffer"
     | Callback uu___ -> "Callback"
     | Format uu___ -> "Format"
+    | Cancel uu___ -> "Cancel"
 let (query_needs_current_module : query' -> Prims.bool) =
   fun uu___ ->
     match uu___ with
@@ -346,7 +515,8 @@ let (interactive_protocol_features : Prims.string Prims.list) =
   "interrupt";
   "progress";
   "full-buffer";
-  "format"]
+  "format";
+  "cancel"]
 let (json_of_issue_level :
   FStar_Errors.issue_level -> FStar_Compiler_Util.json) =
   fun i ->
@@ -401,3 +571,67 @@ let (json_of_issue : FStar_Errors.issue -> FStar_Compiler_Util.json) =
         uu___1 in
     FStar_Compiler_Effect.op_Less_Bar
       (fun uu___1 -> FStar_Compiler_Util.JsonAssoc uu___1) uu___
+let (js_pushkind : FStar_Compiler_Util.json -> push_kind) =
+  fun s ->
+    let uu___ = FStar_Interactive_JsonHelper.js_str s in
+    match uu___ with
+    | "syntax" -> SyntaxCheck
+    | "lax" -> LaxCheck
+    | "full" -> FullCheck
+    | uu___1 -> FStar_Interactive_JsonHelper.js_fail "push_kind" s
+let (js_reductionrule :
+  FStar_Compiler_Util.json -> FStar_TypeChecker_Env.step) =
+  fun s ->
+    let uu___ = FStar_Interactive_JsonHelper.js_str s in
+    match uu___ with
+    | "beta" -> FStar_TypeChecker_Env.Beta
+    | "delta" ->
+        FStar_TypeChecker_Env.UnfoldUntil FStar_Syntax_Syntax.delta_constant
+    | "iota" -> FStar_TypeChecker_Env.Iota
+    | "zeta" -> FStar_TypeChecker_Env.Zeta
+    | "reify" -> FStar_TypeChecker_Env.Reify
+    | "pure-subterms" -> FStar_TypeChecker_Env.PureSubtermsWithinComputations
+    | uu___1 -> FStar_Interactive_JsonHelper.js_fail "reduction rule" s
+let (js_optional_completion_context :
+  FStar_Compiler_Util.json FStar_Pervasives_Native.option ->
+    completion_context)
+  =
+  fun k ->
+    match k with
+    | FStar_Pervasives_Native.None -> CKCode
+    | FStar_Pervasives_Native.Some k1 ->
+        let uu___ = FStar_Interactive_JsonHelper.js_str k1 in
+        (match uu___ with
+         | "symbol" -> CKCode
+         | "code" -> CKCode
+         | "set-options" -> CKOption false
+         | "reset-options" -> CKOption true
+         | "open" -> CKModuleOrNamespace (true, true)
+         | "let-open" -> CKModuleOrNamespace (true, true)
+         | "include" -> CKModuleOrNamespace (true, false)
+         | "module-alias" -> CKModuleOrNamespace (true, false)
+         | uu___1 ->
+             FStar_Interactive_JsonHelper.js_fail
+               "completion context (code, set-options, reset-options, open, let-open, include, module-alias)"
+               k1)
+let (js_optional_lookup_context :
+  FStar_Compiler_Util.json FStar_Pervasives_Native.option -> lookup_context)
+  =
+  fun k ->
+    match k with
+    | FStar_Pervasives_Native.None -> LKSymbolOnly
+    | FStar_Pervasives_Native.Some k1 ->
+        let uu___ = FStar_Interactive_JsonHelper.js_str k1 in
+        (match uu___ with
+         | "symbol-only" -> LKSymbolOnly
+         | "code" -> LKCode
+         | "set-options" -> LKOption
+         | "reset-options" -> LKOption
+         | "open" -> LKModule
+         | "let-open" -> LKModule
+         | "include" -> LKModule
+         | "module-alias" -> LKModule
+         | uu___1 ->
+             FStar_Interactive_JsonHelper.js_fail
+               "lookup context (symbol-only, code, set-options, reset-options, open, let-open, include, module-alias)"
+               k1)
